FY/Semantics.v
@@ -1,15 +1,19 @@
 From FY Require Export Map.
 From FY Require Export Syntax.
+From FY Require Export Qubit.
 From Coq Require Import Bool.Bool.
 From Coq Require Import Init.Nat.
 From Coq Require Import Arith.Arith.
 From Coq Require Import Arith.EqNat.
 
-Definition state := total_map nat.
-Definition empty_st := (_ !-> 0).
+
+Definition state := total_map R.
+Definition empty_st := (_ !-> 0%R).
 Notation "x '!->' v" := (t_update empty_st x v) (at level 100).
 
-Fixpoint aeval (st : state) (a : arith_exp) : nat :=
+Check ANum.
+
+Fixpoint aeval (st : state) (a : arith_exp) : R :=
   match a with
   | ANum n => n
   | AId x => st x
@@ -19,14 +23,37 @@ Fixpoint aeval (st : state) (a : arith_exp) : nat :=
   | <{a1 / a2}> => (aeval st a1) / (aeval st a2)
   end.
 
-Fixpoint beval (st : state) (b : bool_exp) : bool :=
+Fixpoint beval (st : state) (b : bool_exp) : Prop :=
   match b with
-  | <{true}> => true
-  | <{false}> => false
-  | <{a1 = a2}> => (aeval st a1) =? (aeval st a2)
-  | <{a1 <= a2}> => (aeval st a1) <=? (aeval st a2)
-  | <{~ b1}> => negb (beval st b1)
-  | <{b1 && b2}> => andb (beval st b1) (beval st b2)
+  | <{true}> => True
+  | <{false}> => False
+  | <{a1 = a2}> => (aeval st a1) = (aeval st a2)
+  | <{a1 <= a2}> => (aeval st a1) <= (aeval st a2)
+  | <{~ b1}> => ~ (beval st b1)
+  | <{b1 && b2}> => (beval st b1) /\ (beval st b2)
+  end.
+
+Definition pad (n to dim : nat) (U : Unitary (2^n)) : Unitary (2^dim) :=
+  if (to + n <=? dim)%nat
+  then I (2^to) ⊗ U ⊗ I (2^(dim - n - to))
+  else Zero (2^dim) (2^dim).
+
+Definition eval_cnot (dim m n: nat) : Unitary (2^dim) :=
+  if (m + 1 =? n) then
+    pad 2 m dim CNOT
+  else if (n + 1 =? m) then
+    pad 2 n dim CNOT
+  else
+    Zero _ _.
+
+Definition geval {n} (dim : nat) (g : gate_exp) : Unitary (2^dim) :=
+  match g with
+  | GI j => pad n j dim (I 2)
+  | GH j => pad n j dim H
+  | GX j => pad n j dim X
+  | GZ j => pad n j dim Z
+  | GY j => pad n j dim Y
+  | GCNOT j k => eval_cnot dim j k
   end.
 
 Reserved Notation
@@ -44,18 +71,18 @@ Inductive ceval : com -> state -> state -> Prop :=
       st' =[ c2 ]=> st'' ->
       st =[ c1 ; c2 ]=> st''
   | E_IfTrue : forall  st st' b c1 c2,
-      beval st b = true ->
+      beval st b = True ->
       st =[ c1 ]=> st' ->
       st =[ if b then c1 else c2 end]=> st'
   | E_IfFalse : forall  st st' b c1 c2,
-      beval st b = false ->
+      beval st b = False ->
       st =[ c2 ]=> st' ->
       st =[ if b then c1 else c2 end]=> st'
   | E_WhileFalse : forall  b st c,
-      beval st b = false ->
+      beval st b = False ->
       st =[ while b do c end ]=> st
   | E_WhileTrue : forall  st st' st'' b c,
-      beval st b = true ->
+      beval st b = True ->
       st =[ c ]=> st' ->
       st' =[ while b do c end ]=> st'' ->
       st =[ while b do c end ]=> st''
