README.md
@@ -1,1 +1,3 @@
 # quantum-hoare-logic
+
+Run ###make to compile the files.
